Reduce cheats in `pure_letrec_lamProofTheory`

compiler/backend/proofs/pure_letrec_lamProofScript.sml
@@ -13,14 +13,14 @@ val _ = new_theory "pure_letrec_lamProof";
 
 Definition apps_ok_def:
   apps_ok (apps : string |-> exp) ⇔
-    (* each subtition replaces a ‘Var n’ by ‘App (Var n) arg’ *)
+    (* each substition replaces a ‘Var n’ by ‘App (Var n) arg’ *)
     ∀n v. FLOOKUP apps n = SOME v ⇒ ∃arg. v = App (Var n) arg ∧ closed arg
 End
 
 Definition lams_ok_def:
   lams_ok apps xs ys ⇔
     (* all the substitions in apps must be within set of defined names *)
-    FDOM apps SUBSET set (MAP FST xs) ∧
+    FDOM apps ⊆ set (MAP FST xs) ∧
     LIST_REL
       (λ(v1,x1) (v2,x2).
          (* bound names stay the same *)
@@ -29,23 +29,108 @@ Definition lams_ok_def:
            (* if this is an updated binding, then add a Lam, and subst apps: *)
            ∃w. ~(MEM w (freevars x1)) ∧ ~(MEM w (MAP FST xs)) ∧
                x2 = Lam w (subst apps x1)
-         else (* otherise only subst apps: *) x2 = subst apps x1)
+         else (* otherwise only subst apps: *) x2 = subst apps x1)
       xs ys
 End
 
 Inductive letrec_lam:
   (∀xs x apps ys.
-     apps_ok apps ∧ lams_ok apps xs ys ⇒
+     apps_ok apps ∧ lams_ok apps xs ys ∧ closed (Letrec xs x) ⇒
      letrec_lam
        (Letrec xs x)
        (Letrec ys (subst apps x)))
   ∧
   (∀xs x apps ys arg.
-     apps_ok apps ∧ lams_ok apps xs ys ∧ closed arg ⇒
+     apps_ok apps ∧ lams_ok apps xs ys ∧
+     closed arg ∧ closed (Letrec xs x) ∧ w ∉ freevars (subst apps x) ⇒
      letrec_lam
        (Letrec xs x)
        (App (Letrec ys (Lam w (subst apps x))) arg))
 End
+
+(********************)
+
+Theorem apps_ok_FRANGE_freevars:
+  ∀apps. apps_ok apps ⇒ ∀v. v ∈ FRANGE apps ⇒ freevars v ⊆ FDOM apps
+Proof
+  rw[apps_ok_def, IN_FRANGE_FLOOKUP] >>
+  last_x_assum drule >> strip_tac >> gvs[FLOOKUP_DEF, closed_def]
+QED
+
+Theorem apps_ok_freevars_subst:
+  ∀apps x. apps_ok apps ⇒ freevars (subst apps x) = (freevars x : string list)
+Proof
+  recInduct subst_ind >> rw[] >> gvs[apps_ok_def, subst_def]
+  >- (CASE_TAC >> simp[] >> first_x_assum drule >> rw[] >> gvs[closed_def])
+  >- (simp[MAP_MAP_o, combinTheory.o_DEF] >> AP_TERM_TAC >> rw[MAP_EQ_f])
+  >- gvs[DOMSUB_FLOOKUP_THM]
+  >- (
+    simp[MAP_MAP_o, combinTheory.o_DEF, LAMBDA_PROD] >> simp[GSYM FST_THM] >>
+    gvs[FDIFF_def, FLOOKUP_DRESTRICT] >>
+    AP_TERM_TAC >> simp[] >> AP_TERM_TAC >> simp[] >>
+    rw[MAP_EQ_f] >> PairCases_on `e` >> gvs[] >> res_tac
+    )
+QED
+
+Triviality lams_ok_imps:
+  ∀apps xs ys. lams_ok apps xs ys ⇒
+  MAP FST xs = MAP FST ys ∧ LENGTH xs = LENGTH ys ∧ FDOM apps ⊆ set (MAP FST xs)
+Proof
+  rw[lams_ok_def] >> gvs[LIST_REL_EL_EQN, MAP_EQ_EVERY2] >> rw[] >>
+  last_x_assum drule >> pairarg_tac >> gvs[] >> pairarg_tac >> gvs[]
+QED
+
+Triviality lams_ok_imp_freevars:
+  ∀apps xs ys.
+    lams_ok apps xs ys ∧ apps_ok apps
+  ⇒ MAP (λ(fn,e). freevars e) xs = MAP (λ(fn,e). freevars e) ys
+Proof
+  rw[MAP_EQ_EVERY2] >> gvs[lams_ok_def, LIST_REL_EL_EQN] >> rw[] >>
+  last_x_assum drule >>
+  pairarg_tac >> simp[] >> pairarg_tac >> simp[] >> strip_tac >>
+  EVERY_CASE_TAC >> gvs[] >>
+  drule apps_ok_freevars_subst >> simp[] >>
+  gvs[EXTENSION] >> rw[] >> metis_tac[]
+QED
+
+Theorem letrec_lam_subst:
+  ∀f x g y.  letrec_lam x y ⇒ letrec_lam (subst f x) (subst g y)
+Proof
+  simp[Once letrec_lam_cases] >> rw[] >> rename1 `Letrec xs x`
+  >- (
+    ntac 2 (DEP_ONCE_REWRITE_TAC[subst_ignore]) >>
+    simp[letrec_lam_cases, PULL_EXISTS] >>
+    irule_at Any EQ_REFL >> simp[] >>
+    imp_res_tac apps_ok_freevars_subst >> simp[] >>
+    drule_all lams_ok_imp_freevars >> strip_tac >> gvs[] >>
+    imp_res_tac lams_ok_imps >> gvs[] >>
+    qmatch_goalsub_abbrev_tac `DISJOINT s` >> qsuff_tac `s = {}` >> gvs[] >>
+    unabbrev_all_tac >> gvs[SUBSET_DIFF_EMPTY, BIGUNION_SUBSET, EVERY_MEM] >>
+    gvs[MEM_MAP, PULL_EXISTS, FORALL_PROD] >> rw[] >>
+    gvs[MEM_EL, PULL_EXISTS] >> Cases_on `EL n ys` >> gvs[] >>
+    last_x_assum drule >> Cases_on `EL n xs` >> gvs[] >> rw[] >>
+    gvs[lams_ok_def, LIST_REL_EL_EQN] >> last_x_assum drule >> simp[] >>
+    strip_tac >> gvs[] >> EVERY_CASE_TAC >> gvs[] >>
+    simp[GSYM SUBSET_INSERT_DELETE]
+    )
+  >- (
+    ntac 2 (DEP_ONCE_REWRITE_TAC[subst_ignore]) >>
+    simp[letrec_lam_cases, PULL_EXISTS] >>
+    irule_at Any EQ_REFL >> simp[] >>
+    imp_res_tac apps_ok_freevars_subst >> simp[] >>
+    drule_all lams_ok_imp_freevars >> strip_tac >> gvs[] >>
+    imp_res_tac lams_ok_imps >> gvs[closed_def] >> rw[] >>
+    qmatch_goalsub_abbrev_tac `DISJOINT s` >> qsuff_tac `s = {}` >> gvs[] >>
+    unabbrev_all_tac >> gvs[SUBSET_DIFF_EMPTY, BIGUNION_SUBSET, EVERY_MEM] >>
+    simp[GSYM SUBSET_INSERT_DELETE] >>
+    gvs[MEM_MAP, PULL_EXISTS, FORALL_PROD] >> rw[] >>
+    gvs[MEM_EL, PULL_EXISTS] >> Cases_on `EL n ys` >> gvs[] >>
+    last_x_assum drule >> Cases_on `EL n xs` >> gvs[] >> rw[] >>
+    gvs[lams_ok_def, LIST_REL_EL_EQN] >> last_x_assum drule >> simp[] >>
+    strip_tac >> gvs[] >> EVERY_CASE_TAC >> gvs[] >>
+    simp[GSYM SUBSET_INSERT_DELETE]
+    )
+QED
 
 Theorem letrec_rel_lam_subst:
   ∀x y.
@@ -53,7 +138,32 @@ Theorem letrec_rel_lam_subst:
     ∀f g. fmap_rel (letrec_rel letrec_lam) f g ⇒
           letrec_rel letrec_lam (subst f x) (subst g y)
 Proof
-  cheat
+  ho_match_mp_tac letrec_rel_ind >> rw[] >>
+  simp[subst_def, Once letrec_rel_cases]
+  >- (
+    gvs[fmap_rel_OPTREL_FLOOKUP] >>
+    last_x_assum (qspec_then `n` mp_tac) >>
+    CASE_TAC >> CASE_TAC >> gvs[] >> simp[Once letrec_rel_cases]
+    )
+  >- (
+    last_x_assum irule >>
+    gvs[fmap_rel_OPTREL_FLOOKUP, DOMSUB_FLOOKUP_THM] >> rw[]
+    )
+  >- (gvs[LIST_REL_EL_EQN] >> rw[EL_MAP]) >>
+  (
+    qexists_tac
+      `MAP (λ(p1,p2). (p1, subst (FDIFF g (set (MAP FST xs1))) p2)) xs1` >>
+    qexists_tac `subst (FDIFF g (set (MAP FST xs1))) y` >> simp[] >>
+    simp[MAP_MAP_o, combinTheory.o_DEF, LAMBDA_PROD] >> simp[GSYM FST_THM] >>
+    first_x_assum (irule_at Any) >> gvs[LIST_REL_EL_EQN, EL_MAP] >> rw[]
+    >- (gvs[fmap_rel_OPTREL_FLOOKUP, FDIFF_def, FLOOKUP_DRESTRICT] >> rw[])
+    >- (
+      last_x_assum drule >> Cases_on `EL n xs` >> Cases_on `EL n xs1` >> gvs[] >>
+      disch_then irule >>
+      gvs[fmap_rel_OPTREL_FLOOKUP, FDIFF_def, FLOOKUP_DRESTRICT] >> rw[]
+      ) >>
+    disj1_tac >> drule letrec_lam_subst >> simp[subst_def]
+  )
 QED
 
 Triviality letrec_rel_lam_subst_single:
@@ -61,7 +171,8 @@ Triviality letrec_rel_lam_subst_single:
   letrec_rel letrec_lam a b ⇒
   letrec_rel letrec_lam (subst s a x) (subst s b y)
 Proof
-  cheat
+  rw[] >> irule letrec_rel_lam_subst >>
+  simp[fmap_rel_OPTREL_FLOOKUP, FLOOKUP_UPDATE] >> rw[]
 QED
 
 Theorem letrec_lam_correct:
@@ -167,8 +278,23 @@ Proof
     \\ unabbrev_all_tac
     \\ pop_assum mp_tac
     \\ simp [Once letrec_lam_cases] \\ rw []
-    \\ ‘closed (subst_funs ys (subst apps y1)) ∧ closed (subst_funs f y)’ by cheat
-    \\ ‘letrec_rel letrec_lam (subst_funs f y) (subst_funs ys (subst apps y1))’ by cheat
+    \\ ‘closed (subst_funs ys (subst apps y1)) ∧ closed (subst_funs f y)’ by (
+        rw[subst_funs_def, bind_def, closed_def] >>
+        once_rewrite_tac[GSYM LIST_TO_SET_EQ_EMPTY] >>
+        DEP_ONCE_REWRITE_TAC[freevars_subst] >>
+        drule apps_ok_freevars_subst >> simp[] >> strip_tac >>
+        simp[FDOM_FUPDATE_LIST, MAP_MAP_o, combinTheory.o_DEF, LAMBDA_PROD] >>
+        simp[GSYM FST_THM, SUBSET_DIFF_EMPTY] >>
+        imp_res_tac lams_ok_imps >> gvs[] >>
+        ho_match_mp_tac IN_FRANGE_FUPDATE_LIST_suff >> simp[] >>
+        simp[MAP_MAP_o, combinTheory.o_DEF, LAMBDA_PROD] >>
+        gvs[EVERY_MEM, MEM_MAP, PULL_EXISTS, FORALL_PROD] >> rw[] >>
+        metis_tac[])
+    \\ ‘letrec_rel letrec_lam (subst_funs f y) (subst_funs ys (subst apps y1))’ by (
+      DEP_REWRITE_TAC[subst_funs_eq_subst] >> simp[] >>
+      imp_res_tac lams_ok_imps >> gvs[] >>
+      cheat (* TODO *)
+      )
     THEN1 (* case 1 of letrec_lam *)
      (rewrite_tac [eval_wh_to_def]
       \\ IF_CASES_TAC THEN1 (gvs [] \\ qexists_tac ‘0’ \\ fs [])
@@ -178,14 +304,265 @@ Proof
     \\ IF_CASES_TAC THEN1 (gvs [] \\ qexists_tac ‘0’ \\ fs [])
     \\ gvs []
     \\ ‘subst_funs ys (Lam w (subst apps y1)) =
-        Lam w (subst_funs ys (subst apps y1))’ by
-          cheat (* because w was chosen so that this is true *)
-    \\ fs [eval_wh_to_def] \\ fs [bind_single_def]
-    \\ simp [closed_subst]
-    \\ last_x_assum irule
-    \\ fs [])
-  \\ rename [‘Prim’]
-  \\ cheat (* ought to be the same as in pure_letrecProof *)
+        Lam w (subst_funs ys (subst apps y1))’ by (
+          simp[subst_funs_def, bind_def] >>
+          reverse IF_CASES_TAC >> gvs[]
+          >- (
+            gvs[flookup_fupdate_list] >>
+            pop_assum mp_tac >> CASE_TAC >> strip_tac >> gvs[] >>
+            imp_res_tac ALOOKUP_MEM >> gvs[EVERY_MEM, MEM_MAP, EXISTS_PROD] >>
+            metis_tac[]
+            ) >>
+          simp[subst_def] >> irule (GSYM subst_fdomsub) >> simp[])
+    \\ fs [eval_wh_to_def] \\ fs [bind_single_def])
+  >- (
+    rename [‘Prim p xs’] >>
+    qpat_x_assum `letrec_rel c _ _` mp_tac >>
+    simp[Once letrec_rel_cases] >> rw[] >>
+    Cases_on `p` >> gvs[eval_wh_to_def]
+    >- (
+      IF_CASES_TAC >> gvs[] >- (qexists_tac `0` >> gvs[]) >>
+      IF_CASES_TAC >> gvs[LIST_REL_EL_EQN] >>
+      `∃x1 x2 x3. xs = [x1;x2;x3]` by (
+        Cases_on `xs` >> gvs[] >> Cases_on `t` >> gvs[] >>
+        Cases_on `t'` >> gvs[] >> Cases_on `t` >> gvs[]
+        ) >>
+      `∃y1 y2 y3. ys = [y1;y2;y3]` by (
+        Cases_on `ys` >> gvs[] >> Cases_on `t` >> gvs[] >>
+        Cases_on `t'` >> gvs[] >> Cases_on `t` >> gvs[]
+        ) >>
+      gvs[] >>
+      first_assum (qspec_then `0` assume_tac) >>
+      first_assum (qspec_then `1` assume_tac) >>
+      first_x_assum (qspec_then `2` assume_tac) >> gvs[] >>
+      gvs[DISJ_IMP_THM, FORALL_AND_THM] >>
+      first_x_assum drule_all >> strip_tac >> gvs[] >>
+      reverse (Cases_on `eval_wh_to (k - 1) x1`) >> gvs[]
+      >- (qexists_tac `ck` >> gvs[])
+      >- (qexists_tac `ck` >> gvs[])
+      >- (qexists_tac `ck` >> gvs[])
+      >- (qexists_tac `ck` >> gvs[]) >>
+      reverse (IF_CASES_TAC) >> gvs[]
+      >- (
+        reverse (IF_CASES_TAC) >> gvs[]
+        >- (
+          qexists_tac `ck` >> gvs[] >>
+          Cases_on `l` >> gvs[] >> Cases_on `ys'` >> gvs[]
+          ) >>
+        last_x_assum drule_all >> strip_tac >> gvs[] >>
+        reverse (Cases_on `eval_wh_to (k - 1) x3`) >> gvs[]
+        >- (
+          qexists_tac `ck'` >>
+          Cases_on `eval_wh_to (ck' + k - 1) y1 = wh_Diverge` >> gvs[] >>
+          drule eval_wh_to_agree >>
+          disch_then (qspec_then `ck + k - 1` assume_tac) >> gvs[]
+          ) >>
+        qspecl_then [`ck + ck' + k - 1`,`y1`,`ck + k - 1`] mp_tac eval_wh_inc >>
+        gvs[] >> strip_tac >>
+        qspecl_then [`ck + ck' + k - 1`,`y3`,`ck' + k - 1`] mp_tac eval_wh_inc >>
+        gvs[] >> strip_tac >>
+        qexists_tac `ck + ck'` >> gvs[]
+        )
+      >- (
+        first_x_assum drule_all >> strip_tac >> gvs[] >>
+        reverse (Cases_on `eval_wh_to (k - 1) x2`) >> gvs[]
+        >- (
+          qexists_tac `ck'` >>
+          Cases_on `eval_wh_to (ck' + k - 1) y1 = wh_Diverge` >> gvs[] >>
+          drule eval_wh_to_agree >>
+          disch_then (qspec_then `ck + k - 1` assume_tac) >> gvs[]
+          ) >>
+        qspecl_then [`ck + ck' + k - 1`,`y1`,`ck + k - 1`] mp_tac eval_wh_inc >>
+        gvs[] >> strip_tac >>
+        qspecl_then [`ck + ck' + k - 1`,`y2`,`ck' + k - 1`] mp_tac eval_wh_inc >>
+        gvs[] >> strip_tac >>
+        qexists_tac `ck + ck'` >> gvs[]
+        )
+      )
+    >- (
+      IF_CASES_TAC >> gvs[] >> qexists_tac `0` >> simp[]
+      )
+    >- (
+      IF_CASES_TAC >> gvs[] >- (qexists_tac `0` >> simp[]) >>
+      IF_CASES_TAC >> gvs[] >> gvs[LIST_REL_EL_EQN] >>
+      `∃x. xs = [x]` by (
+        Cases_on `xs` >> gvs[] >> Cases_on `t` >> gvs[]) >>
+      `∃y. ys = [y]` by (
+        Cases_on `ys` >> gvs[] >> Cases_on `t` >> gvs[]) >>
+      gvs[] >>
+      first_x_assum drule_all >> rw[] >>
+      Cases_on `eval_wh_to (k - 1) x` >> gvs[] >>
+      qexists_tac `ck` >> gvs[] >>
+      IF_CASES_TAC >> gvs[] >>
+      IF_CASES_TAC >> gvs[]
+      )
+    >- (
+      IF_CASES_TAC >> gvs[] >- (qexists_tac `0` >> simp[]) >>
+      IF_CASES_TAC >> gvs[] >> gvs[LIST_REL_EL_EQN] >>
+      `∃x. xs = [x]` by (
+        Cases_on `xs` >> gvs[] >> Cases_on `t` >> gvs[]) >>
+      `∃y. ys = [y]` by (
+        Cases_on `ys` >> gvs[] >> Cases_on `t` >> gvs[]) >>
+      gvs[] >>
+      first_x_assum drule_all >> rw[] >>
+      reverse (Cases_on `eval_wh_to (k - 1) x`) >> gvs[]
+      >- (qexists_tac `ck` >> gvs[])
+      >- (qexists_tac `ck` >> gvs[])
+      >- (qexists_tac `ck` >> gvs[])
+      >- (qexists_tac `ck` >> gvs[]) >>
+      reverse IF_CASES_TAC >> gvs[]
+      >- (qexists_tac `ck` >> gvs[] >> EVERY_CASE_TAC >> gvs[]) >>
+      first_x_assum drule >> rw[] >>
+      last_x_assum drule >> impl_tac
+      >- (
+        gvs[closed_def, NIL_iff_NOT_MEM] >>
+        CCONTR_TAC >> gvs[] >>
+        imp_res_tac eval_wh_to_freevars_SUBSET >> gvs[MEM_MAP]
+        >- (
+          pop_assum kall_tac >> pop_assum mp_tac >> simp[PULL_EXISTS] >>
+          goal_assum drule >> simp[EL_MEM]
+          )
+        >- (
+          pop_assum mp_tac >> simp[PULL_EXISTS] >>
+          goal_assum drule >> simp[EL_MEM]
+          )
+        ) >>
+      rw[] >>
+      reverse (Cases_on `eval_wh_to (k - 1) (EL n l)`) >> gvs[]
+      >- (
+        qexists_tac `ck'` >>
+        Cases_on `eval_wh_to (ck' + k - 1) y = wh_Diverge` >> gvs[] >>
+        drule eval_wh_to_agree >>
+        disch_then (qspec_then `ck + k - 1` (assume_tac o GSYM)) >> gvs[]
+        ) >>
+      qspecl_then [`ck + ck' + k - 1`,`y`,`ck + k - 1`] mp_tac eval_wh_inc >>
+      gvs[] >> strip_tac >>
+      qspecl_then [`ck + ck' + k - 1`,`EL n ys'`,`ck' + k - 1`]
+        mp_tac eval_wh_inc >>
+      gvs[] >> strip_tac >>
+      qexists_tac `ck + ck'` >> gvs[]
+      )
+    >- (
+      IF_CASES_TAC >> gvs[] >- (qexists_tac `0` >> gvs[]) >>
+      CASE_TAC >> gvs[]
+      >- (
+        qsuff_tac `get_atoms (MAP (λa. eval_wh_to (k − 1) a) ys) = NONE`
+        >- (rw[] >> qexists_tac `0` >> simp[]) >>
+        gvs[get_atoms_NONE_eq] >> imp_res_tac LIST_REL_LENGTH >> gvs[] >>
+        csimp[EL_MAP] >> gvs[EL_MAP] >>
+        map_every (fn pat => qpat_x_assum pat mp_tac)
+          [`∀e1. MEM e1 _ ⇒ _`, `n < _`,`eval_wh_to _ _ = _`, `∀m. m < _ ⇒ _`,
+           `EVERY _ _`, `EVERY _ _`, `LENGTH _ = _`] >>
+        qid_spec_tac `n` >>
+        qpat_x_assum `LIST_REL _ _ _` mp_tac >>
+        map_every qid_spec_tac [`ys`,`xs`] >>
+        ho_match_mp_tac LIST_REL_ind >> rw[] >>
+        Cases_on `n` >> gvs[]
+        >- (
+          qexists_tac `0` >> gvs[] >>
+          first_x_assum (qspec_then `h1` mp_tac) >> simp[] >>
+          disch_then drule_all >> rw[] >>
+          CCONTR_TAC >> drule eval_wh_inc >>
+          disch_then (qspec_then `ck + k - 1` mp_tac) >> simp[]
+          ) >>
+        rename1 `n < _` >>
+        Cases_on `eval_wh_to (k - 1) h2 = wh_Diverge`
+        >- (qexists_tac `0` >> simp[]) >>
+        last_x_assum (qspec_then `n` mp_tac) >> simp[IMP_CONJ_THM] >>
+        impl_tac
+        >- (rw[] >> last_x_assum (qspec_then `SUC m` mp_tac) >> simp[]) >>
+        strip_tac >> rename1 `l < _` >>
+        qexists_tac `SUC l` >> simp[] >> rw[] >>
+        Cases_on `m` >> gvs[] >>
+        last_x_assum (qspec_then `0` assume_tac) >> gvs[] >>
+        first_x_assum (qspec_then `h1` mp_tac) >> simp[] >>
+        disch_then drule_all >> strip_tac >>
+        drule eval_wh_to_agree >>
+        disch_then (qspec_then `ck + k - 1` mp_tac) >> rw[] >>
+        metis_tac[]
+        ) >>
+      Cases_on `x` >> gvs[]
+      >- (
+        gvs[get_atoms_SOME_NONE_eq, EL_MAP] >>
+        qsuff_tac
+          `∃ck. get_atoms (MAP (λa. eval_wh_to (ck + k − 1) a) ys) = SOME NONE`
+        >- (rw[] >> qexists_tac `ck` >> simp[]) >>
+        simp[get_atoms_SOME_NONE_eq] >> csimp[EL_MAP] >>
+        imp_res_tac LIST_REL_LENGTH >> gvs[] >> goal_assum drule >>
+        map_every (fn pat => qpat_x_assum pat mp_tac)
+          [`∀e1. MEM e1 _ ⇒ _`, `n < _`,` ∀a. eval_wh_to _ _ ≠ _`,
+           `∀m. m ≤ _ ⇒ _`, `EVERY _ _`, `EVERY _ _`, `LENGTH _ = _`] >>
+        qid_spec_tac `n` >>
+        qpat_x_assum `LIST_REL _ _ _` mp_tac >>
+        map_every qid_spec_tac [`ys`,`xs`] >>
+        ho_match_mp_tac LIST_REL_ind >> rw[] >>
+        Cases_on `n` >> gvs[]
+        >- (
+          pop_assum (qspec_then `h1` mp_tac) >> simp[] >>
+          disch_then drule_all >> strip_tac >>
+          qexists_tac `ck` >>
+          Cases_on `eval_wh_to (k - 1) h1` >> gvs[]
+          ) >>
+        rename1 `SUC n` >>
+        last_x_assum (qspec_then `n` mp_tac) >> simp[] >> impl_tac
+        >- (rw[] >> last_x_assum (qspec_then `SUC m` mp_tac) >> simp[]) >>
+        strip_tac >>
+        first_x_assum (qspec_then `h1` mp_tac) >> simp[] >>
+        disch_then drule_all >> strip_tac >>
+        qexists_tac `ck + ck'` >> rw[]
+        >- (
+          qpat_x_assum `∀a. _ ≠ wh_Atom a` (qspec_then `a` mp_tac) >>
+          first_x_assum (qspec_then `n` mp_tac) >> simp[] >> strip_tac >>
+          drule eval_wh_inc >>
+          disch_then (qspec_then `ck + (ck' + k) - 1` assume_tac) >> gvs[]
+          ) >>
+        Cases_on `m` >> gvs[]
+        >- (
+          qspecl_then [`ck + (ck' + k) - 1`,`h2`,`ck' + k - 1`]
+            assume_tac eval_wh_inc >>
+          gvs[] >>
+          full_case_tac >> gvs[] >>
+          last_x_assum (qspec_then `0` assume_tac) >> gvs[]
+          )
+        >- (
+          rename1 `m ≤ _` >>
+          first_x_assum drule >> strip_tac >>
+          drule eval_wh_inc >>
+          disch_then (qspec_then `ck + (ck' + k) - 1` assume_tac) >> gvs[]
+          )
+        ) >>
+      rename1 `SOME (SOME as)` >>
+      qsuff_tac
+        `∃ck. get_atoms (MAP (λa. eval_wh_to (ck + k − 1) a) ys) = SOME (SOME as)`
+      >- (rw[] >> qexists_tac `ck` >> simp[] >> CASE_TAC >> gvs[]) >>
+      gvs[get_atoms_SOME_SOME_eq, EVERY2_MAP] >>
+      map_every (fn pat => qpat_x_assum pat mp_tac)
+        [`∀e1. MEM e1 _ ⇒ _`, `LIST_REL _ _ _`, `EVERY _ _`, `EVERY _ _`] >>
+      qid_spec_tac `as` >>
+      qpat_x_assum `LIST_REL _ _ _` mp_tac >>
+      map_every qid_spec_tac [`ys`,`xs`] >>
+      ho_match_mp_tac LIST_REL_strongind >> rw[] >>
+      rename1 `LIST_REL _ _ as` >>
+      qsuff_tac
+        `∃ck. LIST_REL (λa a'. eval_wh_to (ck + k − 1) a = wh_Atom a') ys as`
+      >- (
+        pop_assum (qspec_then `h1` mp_tac) >> simp[] >>
+        disch_then drule_all >> rw[] >>
+        qexists_tac `ck + ck'` >>
+        qspecl_then [`ck + ck' + k - 1`,`h2`,`ck + k - 1`]
+          assume_tac eval_wh_inc >>
+        gvs[LIST_REL_EL_EQN] >> rw[] >>
+        qspecl_then [`ck + ck' + k - 1`,`EL n ys`,`ck' + k - 1`]
+          assume_tac eval_wh_inc >>
+        gvs[]
+        ) >>
+      last_x_assum irule >> simp[]
+      )
+    >- (
+      IF_CASES_TAC >> gvs[] >- (qexists_tac `0` >> gvs[]) >>
+      IF_CASES_TAC >> gvs[] >> IF_CASES_TAC >> gvs[]
+      )
+    )
 QED
 
 val _ = export_theory();
